Major changes: - Open set is empty everywhere - Invariant is inductive over program transitions and constructors are the initial condition - Consequently, invariants must hold by the end of the first constructor phase - VCs removed to retain performance of non-invariant-utilizing code (see Performance.dfy)

Source/DafnyCore/Resolver/InvariantVisitor.cs
@@ -18,4 +18,6 @@ class InvariantVisitor(ModuleResolver resolver) : ASTVisitor<InvariantVisitor.In
     }
     return true;
   }
+  
+  // NB: InvariantRewriter checks that invariant-bearing classes have at least one constructor; easier to do it post-resolution
 }
