Source/DafnyCore/Rewriters/InvariantRewriter.cs
@@ -1,0 +1,14 @@
+namespace Microsoft.Dafny;
+
+public class InvariantRewriter(ErrorReporter reporter) : IRewriter(reporter) {
+  internal override void PostResolve(ModuleDefinition moduleDefinition) {
+    foreach (var decl in moduleDefinition.TopLevelDecls) {
+      // If a class has an invariant, then it needs at least one constructor (in whose body the invariant will be asserted)
+      // In order for the invariant to be inductive over the transition system of the program
+      // Otherwise, a false invariant will lead to an inconsistency
+      if (decl is ClassDecl { HasConstructor: false } cd and TopLevelDeclWithMembers { Invariant: not null }) {
+        reporter.Error(MessageSource.Resolver, cd, "a class with an invariant must have at least one user-defined constructor");
+      }
+    }
+  }
+}
