Source/DafnyCore/Verifier/Statements/BoogieGenerator.TrAssignment.cs
@@ -37,9 +37,11 @@ public partial class BoogieGenerator {
     if (options.Get(CommonOptionBag.CheckInvariants)) {
       var tok = lhs.Origin;
       // If fse is being assigned externally and it has an invariant, it better be true after the fact
+      // However, if we're in the first phase of a constructor and fse.Obj == this, then disable invariant checking
       // NB: for somayyas@: logic here is different enough to be separate from AddInvariantBoilerPlate()
-      if (lhs is MemberSelectExpr fse && fse.Member.EnclosingClass is TopLevelDeclWithMembers { Invariant: { } invariant } decl) {
-        // NB: if fse.Member is an inherited member, then decl is already the supertype => invariant is already the overridden member (if at all, which is what we want)
+      if (lhs is MemberSelectExpr fse && fse.Member.EnclosingClass is TopLevelDeclWithMembers { Invariant: { } invariant }) {
+        // NB: if fse.Member is an inherited member, then decl is already the supertype =>
+        //   invariant is already the overridden member (if at all, which is what we want)
         // NB: need to write out the Use here to avoid a malformed Boogie AST
         Expression assertion = new BinaryExpr(tok, BinaryExpr.ResolvedOpcode.Or,
           new BinaryExpr(tok, BinaryExpr.ResolvedOpcode.InSet, fse.Obj,
@@ -47,13 +49,12 @@ public partial class BoogieGenerator {
               program.SystemModuleManager.NonNullObjectSetType(tok))),
           invariant.Mention(tok, fse.Obj, program.SystemModuleManager));
         // fse.Obj in $Open || fse.Obj.invariant()
-        if (codeContext is Constructor ctor && ctor.EnclosingClass.Equals(decl)) {
-          // In case we're in the fse.Obj's constructor, we don't actually want to check the invariant (equivalent to having open += {this} at the top of the constructor)
+        if (codeContext is Constructor ctor && inBodyInitContext) {
+          // Disable checking the invariant if fse.Obj == this
           assertion = new BinaryExpr(tok, BinaryExpr.ResolvedOpcode.Or,
             new BinaryExpr(tok, BinaryExpr.ResolvedOpcode.EqCommon, fse.Obj, new ThisExpr(ctor)),
             assertion);
         }
-        
         builder.Add(TrAssumeCmd(tok, etran.CanCallAssumption(assertion)));
         builder.Add(TrAssertCmdDesc(tok, etran.TrExpr(assertion),
           new ObjectInvariant(Dafny.ObjectInvariant.Kind.Assignment, assertion)));
