Source/IntegrationTests/TestFiles/LitTests/LitTest/invariants/ValidIdiomError.dfy
@@ -1,6 +1,10 @@
 // RUN: %exits-with 4 %verify --type-system-refresh --check-invariants "%s" > "%t"
 // RUN: %diff "%s.expect" "%t"
 
+// The apparent circularity between Valid() and the invariant isn't explicitly caught, but
+// Value(), as written, isn't well-formed (value isn't a nat). If this.invariant() is 
+// asserted in the boy of Value(), then this error converts to a non-termination error
+
 class Nat {
   var value: int
   function Value(): nat
@@ -11,7 +15,8 @@ class Nat {
   predicate Valid()
     reads this
   {
-    assert value >= 0; value >= 0
+    Value() >= 0
   }
   invariant Valid()
+  constructor() { value := 0; }
 }
