Source/IntegrationTests/TestFiles/LitTests/LitTest/invariants/MethodCallInInvariantError.dfy
@@ -5,7 +5,12 @@ class Account {
   var credit: nat
   var debit: nat
   lemma Call()
+    ensures this.invariant()
   {
   }
   invariant (Call(); credit - debit >= 0)
+  constructor() {
+    credit := 0;
+    debit := 0;
+  }
 }
