Source/IntegrationTests/TestFiles/LitTests/LitTest/invariants/TwoPhaseConstructors.dfy
@@ -1,27 +1,31 @@
-// RUN: %verify --type-system-refresh --check-invariants "%s" > "%t"
+// RUN: %exits-with 4 %verify --type-system-refresh --check-invariants "%s" > "%t"
 // RUN: %diff "%s.expect" "%t"
 
 class C {
   var valid: bool
   invariant valid
 
-  constructor SinglePhase() {
-    //assert valid; // error
-    valid := true;
+  constructor SinglePhaseGood() {
+    valid := true; // ok
+  }
+  
+  constructor SinglePhaseError() {
+    valid := false; // error
   }
 
   constructor TwoPhaseGood() {
     valid := true;
-    new;
     valid := false;
+    valid := true;
+    new;
     valid := true;
     foo(this); // no problem, invariant holds by this point
   }
 
   constructor TwoPhaseBad() {
-    new;
-    //foo(this); // error
+    new; // error: invariant doesn't hold by new;
     valid := true;
+    foo(this);
   }
 
   static method foo(c: C) {
